Categorize instructions (changes memory, etc), define reorderability

Reordering.v
@@ -5,14 +5,67 @@ Require Import List.
 Require Import Common.
 Require Import Lang.
 Require Import Memory.
+Require Import State.
 Require Import LoadStore.
 Require Import SmallStep.
+Require Import Behaviors.
 
 Module Ir.
 
 Module Reordering.
 
+(* Checks whether instruction i2 has data dependency on instruction i1.
+   There's no data dependency, reordering 'i1;i2' into 'i2;i1' wouldn't break use-def chain.
+   Note that this function does not check whether bi2 dominates i1.
+   If i1 has no def (e.g. store instruction), this returns false. *)
+Definition has_data_dependency (i1 i2:Ir.Inst.t): bool :=
+  match (Ir.Inst.def i1) with
+  | None => false
+  | Some (r1, _) => (List.existsb (fun r => Nat.eqb r r1) (Ir.Inst.regops i2))
+  end.
 
+(* Is it valid to reorder 'i1;i2' into 'i2;i1'? *)
+Definition inst_reorderable_unidir (i1 i2:Ir.Inst.t): Prop :=
+  (* If there's no data dependency from i1 to i2 *)
+  forall (HNODEP:has_data_dependency i1 i2 = false),
+    (* 'i1;i2' -> 'i2;i1' is allowed *)
+    forall (st0 st1 st2:Ir.Config.t) (* Initial state, state after i1, state after 'i1;i2' *)
+           (e1 e2:Ir.event) (* i1's event, i2's event *)
+           (HWF:Ir.Config.wf st0) (* Well-formedness of st0 *)
+           (HSTEP1:Ir.SmallStep.inst_step st0 i1 (Ir.SmallStep.sr_success e1 st1))
+           (HSTEP2:Ir.SmallStep.inst_step st1 i2 (Ir.SmallStep.sr_success e2 st2)),
+      exists st1' st2' (* state after i2, state after 'i2;i1' *)
+             e1' e2', (* i2's event, i1's event *)
+        Ir.SmallStep.inst_step st0  i2 (Ir.SmallStep.sr_success e1' st1') /\
+        Ir.SmallStep.inst_step st1' i1 (Ir.SmallStep.sr_success e2' st2') /\
+        st2 = st2' /\ (* Final state is the same *)
+        (* Has same event sequence as well. *)
+        List.filter (Ir.not_none) (e1::e2::nil) = List.filter (Ir.not_none) (e1'::e2'::nil).
+
+(* 'i1;i2 <-> i2;i1'. *)
+Definition inst_reorderable (i1 i2:Ir.Inst.t): Prop :=
+  inst_reorderable_unidir i1 i2 /\ inst_reorderable_unidir i2 i1.
+
+
+
+
+
+(* Reordering between ptrtoint/ptrtoint:
+
+   r1 = ptrtoint opptr1 ty1;
+   r2 = ptrtoint opptr2 ty2
+   ->
+   r2 = ptrtoint opptr2 ty2;
+   r1 = ptrtoint opptr1 ty1
+*)
+(*
+Lemma reorder_unidir_ptrtoint_ptrtoint:
+  forall i1 i2 r1 r2 opptr1 opptr2 ty1 ty2
+         (HINST1:i1 = Ir.Inst.iptrtoint r1 opptr1 ty1)
+         (HINST2:i2 = Ir.Inst.iptrtoint r2 opptr2 ty2),
+    inst_reorderable_unidir i1 i2.
+*)
+  
 
 End Reordering.
 
